# 常用公式集

## 三角函数常用公式

> - $$\sin x = \frac{2\tan\frac{x}{2}}{1+\tan^2\frac{x}{2}}$$
>
> - $$\cos x = \frac{1-\tan^2\frac{x}{2}}{1+\tan^2\frac{x}{2}}$$
>
> - $$\tan x = \frac{2\tan\frac{x}{2}}{1-\tan^2\frac{x}{2}}$$
>
> - $$a\sin x + b\cos x = \sqrt{a^2+b^2}\sin(x+y), \tan y = \frac{b}{a}$$
>
> - $$\sin x = \sin(x+2k\pi)$$
>
> - $$\cos x = \cos(x+2k\pi)$$
>
> - $$\tan x = \tan(x+2k\pi)$$
>
> - $$\sin^2 x + \cos^2 x = 1$$
>
> - $$\sin(x+\pi) = -\sin x$$
>
> - $$\cos(x+\pi) = -\cos x$$
>
> - $$\tan(x+\pi) = \tan x$$
>
> - $$\sin(-x) = -\sin x$$
>
> - $$\cos(-x) = \cos x$$
>
> - $$\tan(-x) = -\tan x$$
>
> - $$\sin(\pi-x) = \sin x$$
>
> - $$\cos(\pi-x) = -\cos x$$
>
> - $$\tan(\pi-x) = -\tan x$$
>
> - $$\sin(\frac{\pi}{2}-x) = \cos x$$
>
> - $$\cos(\frac{\pi}{2}-x) = \sin x$$
>
> - $$\sin(\frac{\pi}{2}+x) = \cos x$$
>
> - $$\cos(\frac{\pi}{2}+x) = -\sin x$$
>
> - $$\cos(x-y) = \cos x \cos y + \sin x \sin y$$
>
> - $$\cos(x+y) = \cos x \cos y - \sin x \sin y$$
>
> - $$\sin(x+y) = \sin x \cos y \pm \cos x \sin y$$
>
> - $$\tan(x+y) = \frac{\tan x + \tan y}{1-\tan x \tan y}$$
>
> - $$\tan(x-y) = \frac{\tan x - \tan y}{1+\tan x \tan y}$$
>
> - $$\sin x + \sin y = 2\sin\frac{x+y}{2}\cos\frac{x-y}{2}$$
>
> - $$\sin x - \sin y = 2\cos\frac{x+y}{2}\sin\frac{x-y}{2}$$
>
> - $$\cos x + \cos y = 2\cos\frac{x+y}{2}\cos\frac{x-y}{2}$$
>
> - $$\cos x - \cos y = -2\sin\frac{x+y}{2}\sin\frac{x-y}{2}$$
>
> - $$\tan x \pm \tan y = \frac{\sin(x \pm y)}{\cos x \cos y}$$
>
> - $$\cot x \pm \cot y = \pm\frac{\sin(x \pm y)}{\sin x \sin y}$$
>
> - $$\sin x \cos y = \frac{1}{2}[\sin(x+y)+\sin(x-y)]$$
>
> - $$\cos x \sin y = \frac{1}{2}[\sin(x+y)-\sin(x-y)]$$
>
> - $$\cos x \cos y = \frac{1}{2}[\cos(x+y)+\cos(x-y)]$$
>
> - $$\sin x \sin y = \frac{1}{2}[\cos(x+y)-\cos(x-y)]$$
>
> - $$\sin2x = 2\sin x\cos x$$
>
> - $$\cos2x = 2\cos^2x-1 = 1-2\sin^2x = \cos^2x-\sin^2x$$
>
> - $$\tan2x = \frac{2\tan x}{1-\tan^2x}$$

## 双曲函数的7个常用公式

> - $$\sh(x+y) = \sh x \ch y + \ch x \sh y$$
>
> - $$\sh(x-y) = \sh x \ch y - \ch x \sh y$$
>
> - $$\ch(x+y) = \ch x \ch y + \sh x \sh y$$
>
> - $$\ch(x-y) = \ch x \ch y - \sh x \sh y$$
>
> - $$\ch^2x-\sh^2x = 1$$
>
> - $$\sh 2x = 2\sh x \ch x$$
>
> - $$\ch 2x = \ch^2x+\sh^2x$$

## 基本初等函数导数公式

> - $$(C)'=0$$
>
> - $$(x^n)'=nx^{n-1}$$
>
> - $$(a^x)'=a^x\ln a$$
>
> - $$(e^x)'=e^x$$
>
> - $$(\log_a{x})'=\frac{1}{x\ln a}$$
>
> - $$(\ln x)' = \frac{1}{x}$$
>
> - $$(\sin x)'=\cos x$$
>
> - $$(\cos x)'=-\sin x$$
>
> - $$(\tan x)'=\sec^2 x$$
>
> - $$(\cot x)'=-\csc^2 x$$
>
> - $$(\sec x)'=\sec x\tan x$$
>
> - $$(\csc x)'=-\csc x\cot x$$
>
> - $$(\arcsin x)' =\frac{1}{\sqrt{1-x^2}}$$
>
> - $$(\arccos x)' =-\frac{1}{\sqrt{1-x^2}}$$
>
> - $$(\arctan x)' =\frac{1}{1+x^2}$$
>
> - $$(arc\cot x)' =-\frac{1}{1+x^2}$$
>
> - $$(\sh x)'=\ch x$$
>
> - $$(\ch x)'=\sh x$$
>
> - $$(\th x)'=\frac{1}{\ch^2x}$$
>
> - $$(ar\sh x)'=\frac{1}{\sqrt{1+x^2}}$$
>
> - $$(ar\ch x)'=\sqrt{x^2-1}$$
>
> - $$(ar\th x)'=\sqrt{1-x^2}$$